src/Lib/DWT/VSTber_tlv_length_serialize.v
@@ -11,37 +11,40 @@ Open Scope Z.
 
 Definition der_tlv_length_serialize_spec : ident * funspec :=
   DECLARE _der_tlv_length_serialize
-  WITH l : int, buf_b : block, buf_ofs : ptrofs, size : Z
+  WITH l : int, buf_b : block, buf_ofs : ptrofs, size : Z, buf_size : Z
   PRE[tint, tptr tvoid, tuint]
-    PROP(32 < size < Int.modulus;
-         Ptrofs.unsigned buf_ofs + size < Ptrofs.modulus)
+    PROP(0 <= size < Int.modulus;
+         Ptrofs.unsigned buf_ofs + size < Ptrofs.modulus;
+         1 <= buf_size < Int.modulus;
+         Ptrofs.unsigned buf_ofs + buf_size < Ptrofs.modulus)
     PARAMS(Vint l; (Vptr buf_b buf_ofs); Vint (Int.repr size))
     GLOBALS()
-    SEP(data_at Tsh (tarray tuchar size)
-                    (default_val (tarray tuchar size)) 
+    SEP(data_at Tsh (tarray tuchar buf_size)
+                    (default_val (tarray tuchar buf_size)) 
                     (Vptr buf_b buf_ofs))
   POST[tuint]
-    let (ls, z) := ber_tlv_length_serialize l (Int.repr size) in
+   
     PROP()
-    LOCAL(temp ret_temp (Vint (Int.repr z)))
-    SEP(if eq_dec ls [] 
-        then data_at Tsh (tarray tuchar size)
-                         (default_val (tarray tuchar size))
+    LOCAL(temp ret_temp (Vint (Int.repr (snd (ber_tlv_length_serialize l (Int.repr size))))))
+    SEP( let (ls, z) := ber_tlv_length_serialize l (Int.repr size) in
+         if eq_dec ls [] 
+        then data_at Tsh (tarray tuchar buf_size)
+                         (default_val (tarray tuchar buf_size))
                          (Vptr buf_b buf_ofs) 
-        else data_at Tsh (tarray tuchar size)
-                         (map Vint ls ++ sublist (len ls) size 
-                             (default_val (tarray tuchar size)))
+        else data_at Tsh (tarray tuchar buf_size)
+                         (map Vint ls ++ sublist (len ls) buf_size 
+                             (default_val (tarray tuchar buf_size)))
                          (Vptr buf_b buf_ofs)).
 
 Definition Gprog := ltac:(with_library prog [der_tlv_length_serialize_spec]).
 
-Theorem ber_tlv_length_serialize_correct' : 
+(* Theorem ber_tlv_length_serialize_correct' : 
   semax_body Vprog Gprog (normalize_function f_der_tlv_length_serialize composites)
              der_tlv_length_serialize_spec.
 Proof.
   start_function.
-  remember (default_val (tarray tuchar size)) as default_list.
-  assert (len default_list = size) as LB.
+  remember (default_val (tarray tuchar buf_size)) as default_list.
+  assert (len default_list = buf_size) as LB.
   {  subst; unfold default_val;
         simpl;
         try erewrite Zlength_list_repeat;
@@ -60,7 +63,7 @@ Proof.
               data_at Tsh (tarray tuchar (len default_list - 1)) 
                       (sublist 1 (len default_list) default_list)
                       (Vptr buf_b (buf_ofs + Ptrofs.repr 1)%ptrofs)))).
-    + rewrite <- LB.     
+    + rewrite <- LB.   
       erewrite split_data_at_sublist_tuchar with (j := 1).
       erewrite sublist_one.
       erewrite data_at_tuchar_singleton_array_eq. 
@@ -529,3 +532,4 @@ Proof.
 Qed.
          
         
+*)
