src/Lib/DWT/VSTder_write_TL.v
@@ -1,0 +1,216 @@
+Require Import Core.Core Core.VstTactics Core.StructNormalizer VstLib
+        ErrorWithWriter.
+Require Import Core.Tactics.
+               
+Require Import VST.floyd.proofauto.
+Require Import Clight.der_encoder.
+Require Import Core.Notations Core.SepLemmas.
+Require Import Clight.dummy Lib.Callback.Dummy ExecBer_tlv_tag_serialize
+        ExecBer_tlv_length_serialize.
+Require Import VSTber_tlv_length_serialize
+        VSTber_tlv_tag_serialize.
+
+Definition Vprog : varspecs. mk_varspecs prog. Defined.
+Instance CompSpecs : compspecs. make_compspecs prog. Defined.
+
+Instance Change1 : change_composite_env CompSpecs  VSTber_tlv_tag_serialize.CompSpecs.
+Proof. make_cs_preserve CompSpecs  VSTber_tlv_tag_serialize.CompSpecs. Defined.
+
+Instance Change2 : change_composite_env  VSTber_tlv_tag_serialize.CompSpecs CompSpecs.
+Proof. make_cs_preserve  VSTber_tlv_tag_serialize.CompSpecs CompSpecs. Defined.
+
+Open Scope Z.
+
+Definition der_write_TL tag len size := 
+  let (_, t) := ber_tlv_tag_serialize tag (Int.repr size) in
+  let (_, l) := ber_tlv_length_serialize len (Int.repr size) in
+  if ((t =? -1) || (t >? 32))%bool 
+  then -1
+  else if l =? -1 
+       then -1 
+       else let s := l + t in
+            if s >? 32 
+            then -1
+            else s.
+
+
+Lemma tag_serialize_bounds : forall t l, 0 <= snd (ber_tlv_tag_serialize t l) <= 32.
+      { unfold ber_tlv_tag_serialize.
+        intros.
+        cbn.
+        repeat break_if; autorewrite with norm; try nia. } 
+Qed.
+  
+Definition der_write_TL_spec : ident * funspec :=
+  DECLARE _der_write_TL
+  WITH tag : int, len : int, cb : val, app_key : val, constructed : int
+  PRE[tuint, tint, tptr cb_type, tptr tvoid, tint]
+    PROP()
+    PARAMS(Vint tag; Vint len; cb; app_key; Vint constructed)
+    GLOBALS()
+    SEP(data_at_ Tsh enc_key_s app_key;
+        valid_pointer cb)
+  POST[tint]
+    let size := if Val.eq cb nullval then 0 else 32 in
+    let r := der_write_TL tag len size in
+    PROP() 
+    LOCAL(temp ret_temp (Vint (Int.repr r)))
+    SEP(data_at_ Tsh enc_key_s app_key;
+        valid_pointer cb).
+
+Definition Gprog := ltac:(with_library prog [der_write_TL_spec;
+                         ber_tlv_tag_serialize_spec; der_tlv_length_serialize_spec]).
+
+Open Scope Z.
+
+Definition Z_of_val v := 
+  match v with
+  | Vptr b i => Ptrofs.unsigned i 
+  | _ => 0
+  end.
+
+Theorem der_write_TL_serialize_correct : 
+  semax_body Vprog Gprog (normalize_function f_der_write_TL composites)
+             der_write_TL_spec.
+Proof.
+  start_function.
+  forward.
+  forward_if 
+ (PROP (isptr v_buf;
+        Z_of_val v_buf + 32 < Ptrofs.modulus)
+  LOCAL (temp der_encoder._t'1 
+              (if Val.eq cb nullval 
+               then Vzero
+               else (Vint (Int.repr (sizeof (tarray tuchar 32)))));
+         temp der_encoder._size (Vint (Int.repr 0)); 
+         lvar _buf (tarray tuchar 32) v_buf;
+         temp _tag (Vint tag); temp _len (Vint len);
+         temp _cb cb; temp _app_key app_key;
+         temp _constructed (Vint constructed))
+  SEP (data_at_ Tsh (tarray tuchar 32) v_buf;
+       data_at_ Tsh enc_key_s app_key; valid_pointer cb)).
+  - forward.
+    unfold isptr in H.
+    repeat break_match;
+    entailer!.
+    discriminate.
+    edestruct HPv_buf.
+    subst. cbv. auto.
+  - forward.
+    entailer!.
+    edestruct HPv_buf.
+    subst. cbv. auto.
+  - repeat forward.
+    unfold isptr in *.
+    destruct v_buf; try contradiction.
+    cbn in H.
+    break_if.
+    (* cb = nullval *)
+    + forward_call (tag, b, i, 0%Z, 32).
+      repeat split; try rep_omega.      
+      remember (snd (ber_tlv_tag_serialize tag (Int.repr 0))) as z.
+      forward_if ((temp _t'3 (if eq_dec (Int.repr z) (Int.repr (-1)) 
+                    then Vint (Int.one)
+                    else
+           (force_val
+         (sem_cast_i2bool
+            (Val.of_bool
+               (Int.repr 32 < Int.repr 
+                                (snd (ber_tlv_tag_serialize tag (Int.repr 0))))%int)))))). 
+      1-2: repeat forward;
+           entailer!;
+           rewrite_if_b;
+           auto;
+           break_if; entailer!. 
+      assert (z = -1) as Z. 
+      {  unfold ber_tlv_tag_serialize in *.
+            break_if;
+              rewrite_if_b; admit. (* SPEC *) }
+      break_if; try congruence.
+      forward_if.
+      repeat forward.
+      rewrite if_true.
+      entailer!.
+      unfold der_write_TL.
+      repeat break_let.     
+      cbn in Z. subst.
+      do 2 f_equal.
+      unfold ber_tlv_tag_serialize.
+      break_if;
+        rewrite_if_b;
+        reflexivity.
+      discriminate.
+    + (* cb <> nullval *)
+     pose proof (tag_serialize_bounds tag (Int.repr 32)) as TL.
+     repeat forward.
+     forward_call (tag, b, i, 32, 32).
+     repeat split; try rep_omega.      
+     remember (snd (ber_tlv_tag_serialize tag (Int.repr 32))) as z.
+     forward_if ((temp _t'3 (if eq_dec (Int.repr z) (Int.repr (-1)) 
+                    then Vint (Int.one)
+                    else
+           (force_val
+         (sem_cast_i2bool
+            (Val.of_bool
+               (Int.repr 32 < Int.repr 
+                                (snd (ber_tlv_tag_serialize tag (Int.repr 32))))%int)))))). 
+      1-2: repeat forward;
+           entailer!;
+           rewrite_if_b;
+           auto;
+           break_if; entailer!. 
+      rewrite if_false.
+      forward_if.
+      repeat forward.
+      normalize in H0.
+      eapply typed_true_of_bool in H0.
+      clear H1.
+      unfold Int.lt in H0.
+      destruct zlt; try congruence.
+      do 2 rewrite Int.signed_repr in l; try rep_omega.
+      normalize in H0.
+      eapply typed_false_of_bool in H0.
+      unfold Int.lt in H0.
+      destruct zlt; try congruence.
+      do 2 rewrite Int.signed_repr in g; try rep_omega.
+      normalize.
+      rewrite if_false.
+      repeat forward.
+      normalize.
+      forward_if (temp _t'4 (Vint (Int.repr (32 - z)))); try congruence.
+      repeat forward.
+      entailer!. 
+      discriminate.
+      forward_call (len, b, (i + Ptrofs.repr z)%ptrofs, (32 - z), (32 - z)).
+      entailer!.
+      normalize.
+    (* unfold ber_tlv_tag_serialize.
+      destruct (30 >=? Int.unsigned (tag >>u Int.repr 2)) eqn: Z.
+      repeat rewrite_if_b.
+      entailer!.
+      admit. (* true *)
+      repeat rewrite_if_b.
+      entailer!.
+      admit. (* true *)
+      normalize.
+      autorewrite with norm.
+      repeat split; try rep_omega.
+      rewrite Int.unsigned_repr; try rep_omega.
+      (* need two buffers, each size 32 *)
+      admit.
+      admit. (* true *)
+      repeat forward.
+      forward_if.
+      repeat forward.
+      entailer!.
+      unfold der_write_TL.
+      repeat break_let.
+      simpl in H0.
+      inversion H0.
+      cbn in H.
+      cbn in H1.
+      admit.
+      entailer!. *)
+Admitted.
+   
+        
